Writing NoUninitDec
--HG--
branch : facade

platform/cito/facade/CompileModule.v
@@ -1,11 +1,84 @@
 Set Implicit Arguments.
 
 Require Import FModule.
+Require Import Compile.
+Require Import Facade.
+Require Import GoodFunction.
+Require Import GoodModule.
 
 Section ADTValue.
 
   Variable ADTValue : Type.
 
   Notation FModule := (@FModule ADTValue).
+
+  Variable module : FModule.
+
+  Require Import String.
+  Local Open Scope string_scope.
+
+  Definition is_good_module_name (s : string) := negb (prefix "_" s).
+
+  Lemma is_good_module_name_sound_cito name : is_good_module_name name = true -> IsGoodModuleName name.
+  Proof.
+    unfold is_good_module_name, IsGoodModuleName.
+    intros; eapply Bool.negb_true_iff; eauto.
+  Qed.
+
+  Variable m_name : string.
+
+  Hypothesis good_name : is_good_module_name m_name = true.
+
+  Notation FName := SyntaxFunc.Name.
+  Notation MName := GoodModule.Name.
+
+  Require Import GoodFunc.
+
+  Lemma compile_GoodFunc f : GoodFunc (compile_op f).
+    admit.
+  Qed.
+
+  Definition compile_func (name : string) (f : FFunction) : GoodFunction.
+    refine
+      ({|
+          Fun := 
+            {|
+              SyntaxFunc.Name := name;
+              SyntaxFunc.Core := compile_op f
+            |};
+          IsGoodFunc := _
+        |}).
+    simpl.
+    eapply compile_GoodFunc.
+  Defined.
+
+  Require Import StringMap.
+  Import StringMap.
+  Require Import StringMapFacts.
+
+  Definition compile_funcs (funs : StringMap.t FFunction) := List.map (uncurry compile_func) (elements funs).
+
+  Lemma NoDup_elements elt (m : StringMap.t elt) : NoDup (List.map fst (elements m)).
+  Proof.
+    eapply NoDupKey_NoDup_fst.
+    eapply elements_3w.
+  Qed.
+
+  Definition compile : GoodModule.
+    refine 
+      ({|
+          Name := m_name;
+          GoodModuleName := _;
+          Functions := compile_funcs (FModule.Functions module);
+          NoDupFuncNames := _
+        |}).
+    eapply is_good_module_name_sound_cito; eauto.
+    unfold compile_funcs.
+    unfold uncurry.
+    rewrite map_map.
+    unfold compile_func.
+    simpl.
+    eapply NoDup_elements.
+  Defined.
 
 End ADTValue.
