platform/cito/NoUninitDec.v
@@ -1,0 +1,131 @@
+Set Implicit Arguments.
+
+Require Import Syntax.
+
+Require Import FreeVarsExpr.
+
+Require Import Option.
+Require Import String.
+Local Open Scope string_scope.
+
+Require Import List.
+Import ListNotations.
+Local Open Scope list_scope.
+
+Module ListNotationsFix.
+  Notation " [ ] " := (@nil _) : list_scope.
+  Notation " [ x , .. , y ] " := (cons x .. (cons y nil) ..) : list_scope.
+  Notation " +[ ] " := (@nil _) : list_scope.
+  Notation " +[ x , .. , y ] " := (cons x .. (cons y nil) ..) : list_scope.
+End ListNotationsFix.
+Import ListNotationsFix.
+
+Require Import StringSet.
+Import StringSet.
+Require Import StringSetFacts.
+Import FSetNotations.
+Import FSetNotationsTrial.
+Local Open Scope fset_scope.
+
+Coercion string2elt (x : string) : elt := x.
+Coercion singleton : elt >-> t.
+
+Fixpoint inits stmt : StringSet.t :=
+  match stmt with
+    | Assign x _ => x
+    | Label x _ => x
+    | Seq a b => inits a + inits b
+    | Skip => []
+    | Syntax.If _ t f => inits t * inits f
+    | While _ _ => []
+    | Syntax.Call x _ _ => default empty (option_map singleton x)
+  end.
+
+Fixpoint uninited_reads inited stmt :=
+  match stmt with
+    | Assign _ e => free_vars e - inited
+    | Label _ _ => []
+    | Seq a b => uninited_reads inited a + uninited_reads (inited + inits a) b
+    | Skip => []
+    | Syntax.If e t f => (free_vars e - inited) + uninited_reads inited t + uninited_reads inited f
+    | While e s => (free_vars e - inited) + uninited_reads inited s
+    | Syntax.Call _ f args => List.fold_left (fun acc e => free_vars e - inited + acc) args (free_vars f - inited)
+  end.
+
+Require Import FuncCore.
+
+Local Open Scope bool_scope.
+
+Definition is_no_uninited_reads (f : FuncCore) := is_empty (uninited_reads (of_list (ArgVars f)) (Body f)).
+
+Definition is_no_uninited (f : FuncCore) := is_no_uninited_reads f && mem (RetVar f) (inits (Body f)).
+
+Require Wf.
+Require Import Bool.
+
+Require Import GeneralTactics2.
+
+Lemma inits_elim stmt : forall x, In x (inits stmt) -> Wf.writes stmt x.
+Proof.
+  induction stmt; simpl; intros x Hin.
+  - eapply empty_iff in Hin; eauto.
+  - eapply union_iff in Hin.
+    destruct Hin as [Hin | Hin].
+    + left; eauto.
+    + right; eauto.
+  - eapply inter_iff in Hin.
+    destruct Hin as [Hin1 Hin2].
+    eauto.
+  - eapply empty_iff in Hin; eauto.
+  - destruct o as [lhs|]; simpl in *.
+    + eapply singleton_iff in Hin.
+      eauto.
+    + eapply empty_iff in Hin; eauto.
+  - eapply singleton_iff in Hin.
+    eauto.
+  - eapply singleton_iff in Hin.
+    eauto.
+Qed.
+
+Lemma uninited_reads_intro' stmt : forall x uninited inited, Wf.reads uninited stmt x -> (forall x, uninited x -> In x inited -> False) -> In x (uninited_reads inited stmt).
+Proof.
+  induction stmt; simpl; intros x uninited inited Hr Hdisj.
+  - eapply empty_iff; eauto.
+  - eapply union_iff.
+    destruct Hr as [Hr1 | Hr2].
+    + left.
+      eauto.
+    + right.
+      eapply IHstmt2; eauto.
+      intros x' Hu Hi.
+      simpl in *.
+      eapply union_iff in Hi.
+      destruct Hu as [Hu Hnw].
+      (*here*)
+Qed.
+
+Lemma uninited_reads_intro stmt : forall x inited, Wf.reads (fun x => ~ List.In x inited) stmt x -> In x (uninited_reads (of_list inited) stmt).
+
+Lemma is_no_uninited_reads_sound f : is_no_uninited_reads f = true -> forall x, ~ Wf.reads (fun x => ~ List.In x (ArgVars f)) (Body f) x.
+Proof.
+  intros Hb x.
+  unfold is_no_uninited_reads in *.
+  nintro.
+  eapply uninited_reads_intro in H.
+  eapply is_empty_iff in Hb.
+  contradict H.
+  eauto.
+Qed.
+
+Lemma is_no_uninited_sound f : is_no_uninited f = true -> Wf.NoUninitialized (ArgVars f) (RetVar f) (Body f).
+Proof.
+  intros Hb.
+  unfold is_no_uninited, Wf.NoUninitialized in *.
+  eapply andb_true_iff in Hb.
+  destruct Hb as [Hnur Hr].
+  split.
+  eapply is_no_uninited_reads_sound; eauto.
+  eapply mem_iff in Hr.
+  eapply inits_elim; eauto.
+Qed.
+
